Fix more init lemmas for txn refinement

src/program_logic/init_cancel.v
@@ -1,5 +1,5 @@
 From iris.proofmode Require Import tactics.
-From Perennial.program_logic Require Export crash_weakestpre.
+From Perennial.program_logic Require Export crash_weakestpre staged_invariant_alt.
 Set Default Proof Using "Type".
 Import uPred.
 
@@ -7,16 +7,42 @@ Section modality.
 Context `{IRISG: !irisGS Λ Σ}.
 
 Definition init_cancel (P Pc : iProp Σ) : iProp Σ :=
-  (∀ e s k Φ Φc,
-    (P -∗ WPC e @ s; k; ⊤ {{ Φ }} {{ Pc -∗ Φc }}) -∗
-    WPC e @ s; k; ⊤ {{ Φ }} {{ Φc }}).
+  (∀ e s k Φ Φc Φc' mj (HLT: (/2 < mj)%Qp),
+    (P -∗ WPC e @ s; k; ⊤ {{ λ v, wpc_crash_modality ⊤ mj (Pc ∗ Φc') -∗ Φ v }} {{ Pc -∗ Φc }}) -∗
+    WPC e @ s; k; ⊤ {{ λ v, wpc_crash_modality ⊤ mj Φc' -∗ Φ v }} {{ Φc }}).
 
 Lemma init_cancel_elim s k e Φ Φc P Pc :
   init_cancel P Pc -∗
   (P -∗ WPC e @ s; k; ⊤ {{ Φ }} {{ Pc -∗ Φc }}) -∗
   WPC e @ s; k; ⊤ {{ Φ }} {{ Φc }}.
 Proof.
-  rewrite /init_cancel. iIntros "H Hwp". iApply "H". eauto.
+  rewrite /init_cancel. iIntros "H Hwp".
+  iAssert (WPC e @ s; k; ⊤ {{ v, wpc_crash_modality ⊤ 1%Qp True%I -∗ Φ v }} {{ Φc }})%I with "[-]" as "H".
+  { unshelve (iApply ("H" $! _ _ _ _ _ True%I 1%Qp _)); eauto.
+    { rewrite //=. }
+    iIntros "HP". iSpecialize ("Hwp" with "[$]").
+    iApply (wpc_mono with "Hwp"); eauto. }
+  iApply (wpc_mono with "H"); eauto.
+  iIntros (?) "H". iApply "H".
+  iApply wpc_crash_modality_intro; eauto.
+Qed.
+
+Lemma init_cancel_elim' s k e Φ Φc P Pc mj :
+  (/2 < mj)%Qp →
+  init_cancel P Pc -∗
+  (P -∗ WPC e @ s; k; ⊤ {{ λ v, wpc_crash_modality ⊤ mj Pc -∗ Φ v }} {{ Pc -∗ Φc }}) -∗
+  WPC e @ s; k; ⊤ {{ Φ }} {{ Φc }}.
+Proof.
+  rewrite /init_cancel. iIntros (?) "H Hwp".
+  iAssert (WPC e @ s; k; ⊤ {{ v, wpc_crash_modality ⊤ mj%Qp True%I -∗ Φ v }} {{ Φc }})%I with "[-]" as "H".
+  { unshelve (iApply ("H" $! _ _ _ _ _ True%I mj%Qp _)); eauto.
+    iIntros "HP". iSpecialize ("Hwp" with "[$]").
+    iApply (wpc_mono with "Hwp"); eauto.
+    iIntros (?) "H Hcm". iApply "H".
+    iApply (wpc_crash_modality_wand with "Hcm"). iIntros "($&_)"; eauto. }
+  iApply (wpc_mono with "H"); eauto.
+  iIntros (?) "H". iApply "H".
+  iApply wpc_crash_modality_intro; eauto.
 Qed.
 
 Lemma init_cancel_sep P1 Pc1 P2 Pc2 :
@@ -26,11 +52,14 @@ Lemma init_cancel_sep P1 Pc1 P2 Pc2 :
 Proof.
   iIntros "Hc1 Hc2".
   rewrite /init_cancel.
-  iIntros (e s k Φ Φc) "Hwp".
-  iApply "Hc1". iIntros "HP1".
-  iApply "Hc2". iIntros "HP2".
+  iIntros (e s k Φ Φc Φc' mj Hlt) "Hwp".
+  iApply ("Hc1" with "[//]"). iIntros "HP1".
+  iApply ("Hc2" with "[//]"). iIntros "HP2".
   iSpecialize ("Hwp" with "[$]").
-  iApply (wpc_mono with "Hwp"); first done.
+  iApply (wpc_mono with "Hwp").
+  { iIntros (?) "H Hwpc". iApply "H".
+    iApply (wpc_crash_modality_wand with "Hwpc").
+    iIntros "($&$&$)". eauto. }
   iIntros "H HPc2 HPc1". iApply "H". by iFrame.
 Qed.
 
@@ -38,24 +67,28 @@ Lemma fupd_init_cancel P Pc :
   (|={⊤}=> init_cancel P Pc) -∗ init_cancel P Pc.
 Proof.
   iIntros "H".
-  iIntros (e s k Φ Φc) "Hwp".
+  iIntros (e s k Φ Φc ???) "Hwp".
   iApply (fupd_wpc).
   iMod "H". iModIntro.
-  iApply "H". eauto.
+  iApply "H"; eauto.
 Qed.
 
 Lemma init_cancel_fupd E P Pc :
   init_cancel (|={E}=> P) (|={E}=> Pc) -∗ init_cancel P Pc.
 Proof.
   iIntros "H".
-  iIntros (e s k Φ Φc) "Hwp".
+  iIntros (e s k Φ Φc ???) "Hwp".
   iApply wpc_cfupd.
-  iApply "H". iIntros "HP".
+  iApply "H"; auto. iIntros "HP".
   iApply (fupd_wpc).
   iMod (fupd_mask_subseteq E) as "Hclo"; first set_solver+.
   iMod "HP". iMod "Hclo". iModIntro.
   iSpecialize ("Hwp" with "[$]").
-  iApply (wpc_mono with "Hwp"); first done.
+  iApply (wpc_mono with "Hwp").
+  { iIntros (?) "H Hcm". iApply "H".
+    iApply (wpc_crash_modality_wand with "Hcm"). iIntros "(H&$)".
+    iMod (fupd_mask_subseteq E) as "Hclo"; first set_solver+.
+    iMod "H". iMod "Hclo". iModIntro. eauto. }
   iIntros "Hc HPC". iIntros "HC".
   iMod (fupd_mask_subseteq E) as "Hclo"; first set_solver+.
   iMod "HPC". iMod "Hclo". iModIntro.
@@ -66,9 +99,11 @@ Lemma init_cancel_intro_l P :
   P -∗ init_cancel P True%I.
 Proof.
   iIntros "HP".
-  iIntros (e s k Φ Φc) "Hwp".
+  iIntros (e s k Φ Φc ???) "Hwp".
   iSpecialize ("Hwp" with "[$]").
-  iApply (wpc_mono with "Hwp"); first done.
+  iApply (wpc_mono with "Hwp").
+  { iIntros (?) "H Hcm". iApply "H".
+    iApply (wpc_crash_modality_wand with "Hcm"). eauto. }
   iIntros "H". iApply "H". eauto.
 Qed.
 
@@ -76,10 +111,12 @@ Lemma init_cancel_intro_r P :
   P -∗ init_cancel True%I P.
 Proof.
   iIntros "HP".
-  iIntros (e s k Φ Φc) "Hwp".
+  iIntros (e s k Φ Φc ???) "Hwp".
   iSpecialize ("Hwp" with "[]"); first done.
   iApply (wpc_strong_mono with "Hwp"); auto.
   iSplit; eauto.
+  { iIntros (?) "H". iModIntro. iIntros "Hcm". iApply "H".
+    iApply (wpc_crash_modality_wand with "Hcm"). iIntros "$"; iFrame. eauto. }
   iIntros "H !>". iApply "H". eauto.
 Qed.
 
@@ -87,10 +124,12 @@ Lemma init_cancel_intro P Pc :
   P -∗ Pc -∗ init_cancel P Pc.
 Proof.
   iIntros "HP HPc".
-  iIntros (e s k Φ Φc) "Hwp".
+  iIntros (e s k Φ Φc ???) "Hwp".
   iSpecialize ("Hwp" with "[$]").
   iApply (wpc_strong_mono with "Hwp"); auto.
   iSplit; eauto.
+  { iIntros (?) "H !> Hcm". iApply "H".
+    iApply (wpc_crash_modality_wand with "Hcm"). iIntros "$". eauto. }
   iIntros "H !>". iApply "H". eauto.
 Qed.
 
@@ -98,11 +137,13 @@ Lemma init_cancel_shift P1 P2 Pc:
   init_cancel (P1 ∗ P2) Pc -∗ init_cancel P1 (Pc ∗ P2).
 Proof.
   iIntros "H".
-  iIntros (e s k Φ Φc) "Hwp".
-  iApply "H". iIntros "(HP1&HP2)".
+  iIntros (e s k Φ Φc ???) "Hwp".
+  iApply "H"; auto. iIntros "(HP1&HP2)".
   iSpecialize ("Hwp" with "[$]").
   iApply (wpc_strong_mono with "Hwp"); auto.
   iSplit; eauto.
+  { iIntros (?) "H !> Hcm". iApply "H".
+    iApply (wpc_crash_modality_wand with "Hcm"). iIntros "($&$)". eauto. }
   iIntros "H !> HPC". iApply "H". by iFrame.
 Qed.
 
@@ -113,13 +154,16 @@ Lemma init_cancel_wand P P' Pc Pc' :
   init_cancel P' Pc'.
 Proof.
   iIntros "H H1 H2".
-  iIntros (e s k Φ Φc) "Hwp".
-  iApply "H". iIntros "HP".
+  iIntros (e s k Φ Φc ???) "Hwp".
+  iApply "H"; auto. iIntros "HP".
   iDestruct ("H1" with "[$]") as "HP".
   iSpecialize ("Hwp" with "[$]").
   iApply (wpc_strong_mono with "[$]"); eauto.
-  iSplit; first eauto. iIntros "H1 !> HPC". iApply "H1". iApply "H2".
-  eauto.
+  iSplit; first eauto.
+  { iIntros (?) "H !> Hcm". iApply "H".
+    iApply (wpc_crash_modality_wand with "Hcm"). iIntros "(H&$)".
+    iApply "H2". eauto. }
+  iIntros "H1 !> HPC". iApply "H1". iApply "H2". eauto.
 Qed.
 
 Lemma big_sepL_init_cancel {A} (Φ Φc : nat → A → iProp Σ) (l : list A) :
